SafetyLemmas.v
@@ -5,17 +5,18 @@ From Elo Require Import TypeProperties.
 
 From Elo Require Import Multistep.
 
+(*
 (* ------------------------------------------------------------------------- *)
 (* one-cr inheritance                                                        *)
 (* ------------------------------------------------------------------------- *)
 
-Lemma onecr_inheritance_rstep :
+Lemma onecr_inheritance_cstep :
   forall ad m1 m2 ths1 ths2 tid tid' e,
     invariants m1 ths1 ->
     invariants m2 ths2 ->
     (* --- *)
-    one_cr ad ths2[tid] ->
-    m1 \ ths1 ~~~[tid', e]~~> m2 \ ths2 ->
+    one_cr ad ths2[tid]                ->
+    m1 \ ths1 ~~[tid', e]~~> m2 \ ths2 ->
     exists t, (e <> e_acq ad t /\ one_cr ad ths1[tid]) \/
               (e =  e_acq ad t /\ tid' = tid).
 Proof.
@@ -23,32 +24,39 @@ Proof.
   assert (forall_memory m1 value) by eauto with inva.
   assert (forall_memory m1 (valid_term m1)) by eauto with inva.
   assert (forall_threads ths1 (valid_term m1)) by eauto with inva.
-  assert (unique_critical_regions m1 ths1) by eauto with inva.
-  assert (Hucr : unique_critical_regions m2 ths2) by eauto with inva.
+  assert (unique_holding m1 ths1) by eauto with inva.
+  assert (Huh : unique_holding m2 ths2) by eauto with inva.
   assert (forall_threads ths1 term_init_cr_exc) by eauto with inva.
   assert (H' : forall_threads ths2 term_init_cr_exc) by eauto with inva.
-  invc_rstep; invc_cstep; try invc_mstep.
+  invc_cstep; try invc_mstep.
   - exists <{unit}>. left. split. 1: intros F; invc F.
     omicron; eauto using onecr_inheritance_none.
   - exists <{unit}>. left. split. 1: intros F; invc F.
     omicron; eauto using onecr_inheritance_alloc.
   - exists <{unit}>. left. split. 1: intros F; invc F.
-    omicron; eauto using onecr_inheritance_insert.
+    omicron; eauto using onecr_inheritance_init.
   - exists <{unit}>. left. split. 1: intros F; invc F.
-    omicron; eauto using nocrs_from_value, onecr_inheritance_read.
+    omicron; eauto using nocr_from_value, onecr_inheritance_read.
   - exists <{unit}>. left. split. 1: intros F; invc F.
     omicron; eauto using onecr_inheritance_write.
-  - exists t.
-    match goal with _ : _ --[e_acq ?ad' _]--> _ |- _ => nat_eq_dec ad' ad end.
-    + omicron; eauto.
+  - exists t'. omicron.
+    + left. split.
+      * intros F. invc F. auto.
+      * omicron; eauto using nocrs_from_value, onecr_inheritance_acq.
+    +
+    + nat_eq_dec ad' ad; eauto.
+      assert (term_init_cr_exc t) by (specialize (H' tid); sigma; trivial).
+      assert (no_cr ad' ths1[tid]) by eauto using nocr_from_acq with inva.
+
+      assert (one_cr ad ths1[tid <- t][tid']) by (sigma; trivial).
+      assert (one_cr ad ths1[tid <- t][tid])  by (sigma; trivial).
+
       match goal with _ : _ --[_]--> ?t |- _ =>
-        assert (term_init_cr_exc t) by (specialize (H' tid'); sigma; trivial);
-        assert (no_cr ad ths1[tid']) by eauto using nocr_from_acq with inva;
-        assert (one_cr ad t) by eauto using nocr_to_onecr, nocrs_from_value;
+        (* assert (one_cr ad t) by eauto using nocr_to_onecr, nocrs_from_value; *)
         assert (one_cr ad ths1[tid' <- t][tid']) by (sigma; trivial);
         assert (one_cr ad ths1[tid' <- t][tid])  by (sigma; trivial)
       end.
-      exfalso. eauto using ucr_onecr_contradiction.
+      exfalso. eauto using uh_onecr_contradiction.
     + left. split.
       * intros F. invc F. auto.
       * omicron; eauto using nocrs_from_value, onecr_inheritance_acq.
@@ -61,45 +69,46 @@ Proof.
     omicron; eauto using onecr_inheritance_spawn.
     exfalso. eauto using nocr_spawn_term, nocr_onecr_contradiction.
 Qed.
+*)
 
 (* ------------------------------------------------------------------------- *)
 (* initialized preservation                                                  *)
 (* ------------------------------------------------------------------------- *)
 
-Lemma initialized_preservation_rstep : forall m1 m2 ths1 ths2 tid e ad t,
-  m1[ad].t = Some t ->
-  m1 \ ths1 ~~~[tid, e]~~> m2 \ ths2 ->
+Lemma initialized_preservation_cstep : forall m1 m2 ths1 ths2 tid e ad t,
+  m1[ad].t = Some t                 ->
+  m1 \ ths1 ~~[tid, e]~~> m2 \ ths2 ->
   exists t', m2 [ad].t = Some t'.
 Proof.
   intros.
   assert (ad < #m1) by (lt_eq_gt ad (#m1); sigma; upsilon; eauto).
-  invc_rstep; invc_cstep; try invc_mstep; sigma; eauto;
+  invc_cstep; try invc_mstep; sigma; eauto;
   omicron; upsilon; eauto.
 Qed.
 
 Lemma initialized_preservation_ustep : forall m1 m2 ths1 ths2 tc ad t,
-  m1[ad].t = Some t ->
+  m1[ad].t = Some t              ->
   m1 \ ths1 ~~[tc]~~>* m2 \ ths2 ->
   exists t', m2 [ad].t = Some t'.
 Proof.
   intros. ind_ustep; eauto.
   destruct IHmultistep; trivial.
-  eauto using initialized_preservation_rstep.
+  eauto using initialized_preservation_cstep.
 Qed.
 
 (* ------------------------------------------------------------------------- *)
 (* one-init preservation                                                     *)
 (* ------------------------------------------------------------------------- *)
 
-Lemma oneinit_preservation_rstep :
+Lemma oneinit_preservation_cstep :
   forall ad m1 m2 ths1 ths2 tid tid' e,
     invariants m1 ths1 ->
     invariants m2 ths2 ->
     (* --- *)
-    one_init ad ths1[tid] ->
-    m1 \ ths1 ~~~[tid', e]~~> m2 \ ths2 ->
-     (forall t, e <> e_insert ad t /\ one_init ad ths2[tid]) \/
-     (exists t, e =  e_insert ad t /\ tid' = tid /\ m2[ad].t = Some t).
+    one_init ad ths1[tid]              ->
+    m1 \ ths1 ~~[tid', e]~~> m2 \ ths2 ->
+     (forall t, e <> e_init ad t /\ one_init ad ths2[tid]) \/
+     (exists t, e =  e_init ad t /\ tid' = tid /\ m2[ad].t = Some t).
 Proof.
   intros.
   assert (forall_memory m1 value) by eauto with inva.
@@ -107,28 +116,32 @@ Proof.
   assert (forall_threads ths1 (valid_term m1)) by eauto with inva.
   assert (forall_threads ths1 (consistent_term m1)) by eauto with inva.
   assert (unique_initializers m1 ths1) by eauto with inva.
-  invc_rstep; invc_cstep; try invc_mstep.
-  - left. intros. split; auto.
+  invc_cstep; try invc_mstep.
+  - left. intros. split; eauto.
     omicron; eauto using oneinit_preservation_none.
-  - left. split; try omicron; auto.
+  - left. split; try omicron; auto; try congruence.
     assert (ad < #m1) by eauto using oneinit_ad_bound.
     eauto using oneinit_preservation_alloc.
-  - match goal with _ : _ --[e_insert ?x _]--> _ |- _ => rename x into ad' end.
+  - match goal with _ : _ --[e_init ?x _]--> _ |- _ => rename x into ad' end.
     nat_eq_dec ad' ad.
-    + assert (ad < #m1) by eauto using vtm_insert_address.
+    + assert (ad < #m1) by eauto using vtm_init_address.
       right. repeat eexists; sigma; upsilon; trivial.
-      eauto using oneinit_from_insert, ui_oneinit_equality.
+      eauto using oneinit_from_init, ui_oneinit_equality.
     + left. intros. split; auto.
-      omicron; eauto using oneinit_preservation_insert.
-  - left. split; auto.
+      omicron; eauto using oneinit_preservation_init.
+  - left. split; auto; try congruence.
     omicron; eauto using noinits_from_value, oneinit_preservation_read.
-  - left. split; auto.
+  - left. split; auto; try congruence.
     omicron; eauto using oneinit_preservation_write.
   - left. split; auto.
     omicron; eauto using noinits_from_value, oneinit_preservation_acq.
   - left. split; auto.
     omicron; eauto using oneinit_preservation_rel.
-  - left. split; auto.
+  - left. split; auto; try congruence.
+    omicron; eauto using oneinit_preservation_wacq.
+  - left. split; auto; try congruence.
+    omicron; eauto using oneinit_preservation_wrel.
+  - left. split; auto; try congruence.
     omicron; eauto using oneinit_preservation_spawn.
     invc_oneinit.
 Qed.
@@ -138,12 +151,12 @@ Lemma oneinit_preservation_ustep :
     invariants m1 ths1 ->
     invariants m2 ths2 ->
     (* --- *)
-    one_init ad ths1[tid] ->
+    one_init ad ths1[tid]          ->
     m1 \ ths1 ~~[tc]~~>* m2 \ ths2 ->
     one_init ad ths2[tid] \/ exists t, m2[ad].t = Some t.
 Proof.
   intros. ind_ustep; auto.
-  match goal with _ : ?m \ ?ths ~~~[?tid, _]~~> ?m' \ ?ths' |- _ =>
+  match goal with _ : ?m \ ?ths ~~[?tid, _]~~> ?m' \ ?ths' |- _ =>
     rename tid into tid';
     rename m' into m3; rename ths' into ths3;
     rename m  into m2; rename ths  into ths2
@@ -151,15 +164,16 @@ Proof.
   assert (invariants m2 ths2) by eauto using invariants_preservation_ustep.
   destruct IHmultistep as [? | [? ?]]; trivial.
   - assert (
-      (forall t, e <> e_insert ad t /\ one_init ad ths3[tid]) \/
-      (exists t, e =  e_insert ad t /\ tid' = tid /\ m3[ad].t = Some t)
+      (forall t, e <> e_init ad t /\ one_init ad ths3[tid]) \/
+      (exists t, e =  e_init ad t /\ tid' = tid /\ m3[ad].t = Some t)
     ) as [H' | [t' [? [? ?]]]]
-      by eauto using oneinit_preservation_rstep.
+      by eauto using oneinit_preservation_cstep.
     + specialize (H' <{unit}>) as [? ?]. eauto.
     + subst. eauto.
-  - right. eauto using initialized_preservation_rstep.
+  - right. eauto using initialized_preservation_cstep.
 Qed.
 
+(*
 (* ------------------------------------------------------------------------- *)
 (* one-cr preservation                                                       *)
 (* ------------------------------------------------------------------------- *)
@@ -185,7 +199,7 @@ Proof.
   - left. split; auto.
     omicron; eauto using onecr_preservation_alloc.
   - left. split; auto.
-    omicron; eauto using onecr_preservation_insert.
+    omicron; eauto using onecr_preservation_init.
   - left. split; auto.
     omicron; eauto using nocrs_from_value, onecr_preservation_read.
   - left. split; auto.
@@ -206,4 +220,4 @@ Proof.
     omicron; eauto using onecr_preservation_spawn.
     invc_onecr.
 Qed.
-
+*)
